DynamoDbEncryptionMiddlewareInternal/runtimes/java/src/main/smithy-generated/software/amazon/cryptography/dynamoDbEncryption/ToNative.java
@@ -10,9 +10,12 @@ import Dafny.Aws.Cryptography.DynamoDbEncryption.Types.Error_Opaque;
 import dafny.DafnyMap;
 import dafny.DafnySequence;
 import java.lang.Character;
+import java.lang.IllegalArgumentException;
+import java.lang.Integer;
 import java.lang.String;
 import java.util.List;
 import java.util.Map;
+import java.util.function.Function;
 import software.amazon.cryptography.dynamoDbEncryption.model.BatchExecuteStatementInputTransformInput;
 import software.amazon.cryptography.dynamoDbEncryption.model.BatchExecuteStatementInputTransformOutput;
 import software.amazon.cryptography.dynamoDbEncryption.model.BatchExecuteStatementOutputTransformInput;
@@ -83,6 +86,7 @@ import software.amazon.cryptography.dynamoDbEncryption.model.TransactWriteItemsI
 import software.amazon.cryptography.dynamoDbEncryption.model.TransactWriteItemsInputTransformOutput;
 import software.amazon.cryptography.dynamoDbEncryption.model.TransactWriteItemsOutputTransformInput;
 import software.amazon.cryptography.dynamoDbEncryption.model.TransactWriteItemsOutputTransformOutput;
+import software.amazon.cryptography.dynamoDbEncryption.model.Transform;
 import software.amazon.cryptography.dynamoDbEncryption.model.UpdateItemInputTransformInput;
 import software.amazon.cryptography.dynamoDbEncryption.model.UpdateItemInputTransformOutput;
 import software.amazon.cryptography.dynamoDbEncryption.model.UpdateItemOutputTransformInput;
@@ -91,6 +95,9 @@ import software.amazon.cryptography.dynamoDbEncryption.model.UpdateTableInputTra
 import software.amazon.cryptography.dynamoDbEncryption.model.UpdateTableInputTransformOutput;
 import software.amazon.cryptography.dynamoDbEncryption.model.UpdateTableOutputTransformInput;
 import software.amazon.cryptography.dynamoDbEncryption.model.UpdateTableOutputTransformOutput;
+import software.amazon.cryptography.dynamoDbEncryption.model.VirtualField;
+import software.amazon.cryptography.dynamoDbEncryption.model.VirtualPart;
+import software.amazon.cryptography.dynamoDbEncryption.model.VirtualTransform;
 
 public class ToNative {
   public static OpaqueError Error(Error_Opaque dafnyValue) {
@@ -129,6 +136,85 @@ public class ToNative {
     return nativeBuilder.build();
   }
 
+  public static ExecuteStatementInputTransformOutput ExecuteStatementInputTransformOutput(
+      Dafny.Aws.Cryptography.DynamoDbEncryption.Types.ExecuteStatementInputTransformOutput dafnyValue) {
+    ExecuteStatementInputTransformOutput.Builder nativeBuilder = ExecuteStatementInputTransformOutput.builder();
+    nativeBuilder.transformedInput(Dafny.Com.Amazonaws.Dynamodb.ToNative.ExecuteStatementInput(dafnyValue.dtor_transformedInput()));
+    return nativeBuilder.build();
+  }
+
+  public static ExecuteTransactionInputTransformInput ExecuteTransactionInputTransformInput(
+      Dafny.Aws.Cryptography.DynamoDbEncryption.Types.ExecuteTransactionInputTransformInput dafnyValue) {
+    ExecuteTransactionInputTransformInput.Builder nativeBuilder = ExecuteTransactionInputTransformInput.builder();
+    nativeBuilder.sdkInput(Dafny.Com.Amazonaws.Dynamodb.ToNative.ExecuteTransactionInput(dafnyValue.dtor_sdkInput()));
+    return nativeBuilder.build();
+  }
+
+  public static DeleteItemOutputTransformOutput DeleteItemOutputTransformOutput(
+      Dafny.Aws.Cryptography.DynamoDbEncryption.Types.DeleteItemOutputTransformOutput dafnyValue) {
+    DeleteItemOutputTransformOutput.Builder nativeBuilder = DeleteItemOutputTransformOutput.builder();
+    nativeBuilder.transformedOutput(Dafny.Com.Amazonaws.Dynamodb.ToNative.DeleteItemOutput(dafnyValue.dtor_transformedOutput()));
+    return nativeBuilder.build();
+  }
+
+  public static QueryOutputTransformInput QueryOutputTransformInput(
+      Dafny.Aws.Cryptography.DynamoDbEncryption.Types.QueryOutputTransformInput dafnyValue) {
+    QueryOutputTransformInput.Builder nativeBuilder = QueryOutputTransformInput.builder();
+    nativeBuilder.sdkOutput(Dafny.Com.Amazonaws.Dynamodb.ToNative.QueryOutput(dafnyValue.dtor_sdkOutput()));
+    nativeBuilder.originalInput(Dafny.Com.Amazonaws.Dynamodb.ToNative.QueryInput(dafnyValue.dtor_originalInput()));
+    return nativeBuilder.build();
+  }
+
+  public static PutItemInputTransformOutput PutItemInputTransformOutput(
+      Dafny.Aws.Cryptography.DynamoDbEncryption.Types.PutItemInputTransformOutput dafnyValue) {
+    PutItemInputTransformOutput.Builder nativeBuilder = PutItemInputTransformOutput.builder();
+    nativeBuilder.transformedInput(Dafny.Com.Amazonaws.Dynamodb.ToNative.PutItemInput(dafnyValue.dtor_transformedInput()));
+    return nativeBuilder.build();
+  }
+
+  public static CreateTableInputTransformOutput CreateTableInputTransformOutput(
+      Dafny.Aws.Cryptography.DynamoDbEncryption.Types.CreateTableInputTransformOutput dafnyValue) {
+    CreateTableInputTransformOutput.Builder nativeBuilder = CreateTableInputTransformOutput.builder();
+    nativeBuilder.transformedInput(Dafny.Com.Amazonaws.Dynamodb.ToNative.CreateTableInput(dafnyValue.dtor_transformedInput()));
+    return nativeBuilder.build();
+  }
+
+  public static DescribeTableInputTransformOutput DescribeTableInputTransformOutput(
+      Dafny.Aws.Cryptography.DynamoDbEncryption.Types.DescribeTableInputTransformOutput dafnyValue) {
+    DescribeTableInputTransformOutput.Builder nativeBuilder = DescribeTableInputTransformOutput.builder();
+    nativeBuilder.transformedInput(Dafny.Com.Amazonaws.Dynamodb.ToNative.DescribeTableInput(dafnyValue.dtor_transformedInput()));
+    return nativeBuilder.build();
+  }
+
+  public static DeleteItemInputTransformInput DeleteItemInputTransformInput(
+      Dafny.Aws.Cryptography.DynamoDbEncryption.Types.DeleteItemInputTransformInput dafnyValue) {
+    DeleteItemInputTransformInput.Builder nativeBuilder = DeleteItemInputTransformInput.builder();
+    nativeBuilder.sdkInput(Dafny.Com.Amazonaws.Dynamodb.ToNative.DeleteItemInput(dafnyValue.dtor_sdkInput()));
+    return nativeBuilder.build();
+  }
+
+  public static GetItemOutputTransformInput GetItemOutputTransformInput(
+      Dafny.Aws.Cryptography.DynamoDbEncryption.Types.GetItemOutputTransformInput dafnyValue) {
+    GetItemOutputTransformInput.Builder nativeBuilder = GetItemOutputTransformInput.builder();
+    nativeBuilder.sdkOutput(Dafny.Com.Amazonaws.Dynamodb.ToNative.GetItemOutput(dafnyValue.dtor_sdkOutput()));
+    nativeBuilder.originalInput(Dafny.Com.Amazonaws.Dynamodb.ToNative.GetItemInput(dafnyValue.dtor_originalInput()));
+    return nativeBuilder.build();
+  }
+
+  public static ExecuteTransactionInputTransformOutput ExecuteTransactionInputTransformOutput(
+      Dafny.Aws.Cryptography.DynamoDbEncryption.Types.ExecuteTransactionInputTransformOutput dafnyValue) {
+    ExecuteTransactionInputTransformOutput.Builder nativeBuilder = ExecuteTransactionInputTransformOutput.builder();
+    nativeBuilder.transformedInput(Dafny.Com.Amazonaws.Dynamodb.ToNative.ExecuteTransactionInput(dafnyValue.dtor_transformedInput()));
+    return nativeBuilder.build();
+  }
+
+  public static ExecuteStatementInputTransformInput ExecuteStatementInputTransformInput(
+      Dafny.Aws.Cryptography.DynamoDbEncryption.Types.ExecuteStatementInputTransformInput dafnyValue) {
+    ExecuteStatementInputTransformInput.Builder nativeBuilder = ExecuteStatementInputTransformInput.builder();
+    nativeBuilder.sdkInput(Dafny.Com.Amazonaws.Dynamodb.ToNative.ExecuteStatementInput(dafnyValue.dtor_sdkInput()));
+    return nativeBuilder.build();
+  }
+
   public static TransactWriteItemsOutputTransformInput TransactWriteItemsOutputTransformInput(
       Dafny.Aws.Cryptography.DynamoDbEncryption.Types.TransactWriteItemsOutputTransformInput dafnyValue) {
     TransactWriteItemsOutputTransformInput.Builder nativeBuilder = TransactWriteItemsOutputTransformInput.builder();
@@ -137,10 +223,446 @@ public class ToNative {
     return nativeBuilder.build();
   }
 
+  public static CreateTableOutputTransformInput CreateTableOutputTransformInput(
+      Dafny.Aws.Cryptography.DynamoDbEncryption.Types.CreateTableOutputTransformInput dafnyValue) {
+    CreateTableOutputTransformInput.Builder nativeBuilder = CreateTableOutputTransformInput.builder();
+    nativeBuilder.sdkOutput(Dafny.Com.Amazonaws.Dynamodb.ToNative.CreateTableOutput(dafnyValue.dtor_sdkOutput()));
+    nativeBuilder.originalInput(Dafny.Com.Amazonaws.Dynamodb.ToNative.CreateTableInput(dafnyValue.dtor_originalInput()));
+    return nativeBuilder.build();
+  }
+
+  public static TransactGetItemsOutputTransformInput TransactGetItemsOutputTransformInput(
+      Dafny.Aws.Cryptography.DynamoDbEncryption.Types.TransactGetItemsOutputTransformInput dafnyValue) {
+    TransactGetItemsOutputTransformInput.Builder nativeBuilder = TransactGetItemsOutputTransformInput.builder();
+    nativeBuilder.sdkOutput(Dafny.Com.Amazonaws.Dynamodb.ToNative.TransactGetItemsOutput(dafnyValue.dtor_sdkOutput()));
+    nativeBuilder.originalInput(Dafny.Com.Amazonaws.Dynamodb.ToNative.TransactGetItemsInput(dafnyValue.dtor_originalInput()));
+    return nativeBuilder.build();
+  }
+
+  public static DescribeTableOutputTransformInput DescribeTableOutputTransformInput(
+      Dafny.Aws.Cryptography.DynamoDbEncryption.Types.DescribeTableOutputTransformInput dafnyValue) {
+    DescribeTableOutputTransformInput.Builder nativeBuilder = DescribeTableOutputTransformInput.builder();
+    nativeBuilder.sdkOutput(Dafny.Com.Amazonaws.Dynamodb.ToNative.DescribeTableOutput(dafnyValue.dtor_sdkOutput()));
+    nativeBuilder.originalInput(Dafny.Com.Amazonaws.Dynamodb.ToNative.DescribeTableInput(dafnyValue.dtor_originalInput()));
+    return nativeBuilder.build();
+  }
+
   public static CreateTableInputTransformInput CreateTableInputTransformInput(
       Dafny.Aws.Cryptography.DynamoDbEncryption.Types.CreateTableInputTransformInput dafnyValue) {
     CreateTableInputTransformInput.Builder nativeBuilder = CreateTableInputTransformInput.builder();
     nativeBuilder.sdkInput(Dafny.Com.Amazonaws.Dynamodb.ToNative.CreateTableInput(dafnyValue.dtor_sdkInput()));
+    return nativeBuilder.build();
+  }
+
+  public static CreateTableOutputTransformOutput CreateTableOutputTransformOutput(
+      Dafny.Aws.Cryptography.DynamoDbEncryption.Types.CreateTableOutputTransformOutput dafnyValue) {
+    CreateTableOutputTransformOutput.Builder nativeBuilder = CreateTableOutputTransformOutput.builder();
+    nativeBuilder.transformedOutput(Dafny.Com.Amazonaws.Dynamodb.ToNative.CreateTableOutput(dafnyValue.dtor_transformedOutput()));
+    return nativeBuilder.build();
+  }
+
+  public static GetItemInputTransformOutput GetItemInputTransformOutput(
+      Dafny.Aws.Cryptography.DynamoDbEncryption.Types.GetItemInputTransformOutput dafnyValue) {
+    GetItemInputTransformOutput.Builder nativeBuilder = GetItemInputTransformOutput.builder();
+    nativeBuilder.transformedInput(Dafny.Com.Amazonaws.Dynamodb.ToNative.GetItemInput(dafnyValue.dtor_transformedInput()));
+    return nativeBuilder.build();
+  }
+
+  public static ExecuteTransactionOutputTransformInput ExecuteTransactionOutputTransformInput(
+      Dafny.Aws.Cryptography.DynamoDbEncryption.Types.ExecuteTransactionOutputTransformInput dafnyValue) {
+    ExecuteTransactionOutputTransformInput.Builder nativeBuilder = ExecuteTransactionOutputTransformInput.builder();
+    nativeBuilder.sdkOutput(Dafny.Com.Amazonaws.Dynamodb.ToNative.ExecuteTransactionOutput(dafnyValue.dtor_sdkOutput()));
+    nativeBuilder.originalInput(Dafny.Com.Amazonaws.Dynamodb.ToNative.ExecuteTransactionInput(dafnyValue.dtor_originalInput()));
+    return nativeBuilder.build();
+  }
+
+  public static TransactGetItemsInputTransformOutput TransactGetItemsInputTransformOutput(
+      Dafny.Aws.Cryptography.DynamoDbEncryption.Types.TransactGetItemsInputTransformOutput dafnyValue) {
+    TransactGetItemsInputTransformOutput.Builder nativeBuilder = TransactGetItemsInputTransformOutput.builder();
+    nativeBuilder.transformedInput(Dafny.Com.Amazonaws.Dynamodb.ToNative.TransactGetItemsInput(dafnyValue.dtor_transformedInput()));
+    return nativeBuilder.build();
+  }
+
+  public static QueryInputTransformOutput QueryInputTransformOutput(
+      Dafny.Aws.Cryptography.DynamoDbEncryption.Types.QueryInputTransformOutput dafnyValue) {
+    QueryInputTransformOutput.Builder nativeBuilder = QueryInputTransformOutput.builder();
+    nativeBuilder.transformedInput(Dafny.Com.Amazonaws.Dynamodb.ToNative.QueryInput(dafnyValue.dtor_transformedInput()));
+    return nativeBuilder.build();
+  }
+
+  public static VirtualPart VirtualPart(
+      Dafny.Aws.Cryptography.DynamoDbEncryption.Types.VirtualPart dafnyValue) {
+    VirtualPart.Builder nativeBuilder = VirtualPart.builder();
+    nativeBuilder.loc(software.amazon.dafny.conversion.ToNative.Simple.String(dafnyValue.dtor_loc()));
+    if (dafnyValue.dtor_trans().is_Some()) {
+      nativeBuilder.trans(ToNative.VirtualTransformList(dafnyValue.dtor_trans().dtor_value()));
+    }
+    return nativeBuilder.build();
+  }
+
+  public static VirtualTransform VirtualTransform(
+      Dafny.Aws.Cryptography.DynamoDbEncryption.Types.VirtualTransform dafnyValue) {
+    VirtualTransform.Builder nativeBuilder = VirtualTransform.builder();
+    nativeBuilder.transform(ToNative.Transform(dafnyValue.dtor_transform()));
+    if (dafnyValue.dtor_numbers().is_Some()) {
+      nativeBuilder.numbers(ToNative.NumberList(dafnyValue.dtor_numbers().dtor_value()));
+    }
+    if (dafnyValue.dtor_strings().is_Some()) {
+      nativeBuilder.strings(ToNative.StringList(dafnyValue.dtor_strings().dtor_value()));
+    }
+    return nativeBuilder.build();
+  }
+
+  public static BatchExecuteStatementInputTransformInput BatchExecuteStatementInputTransformInput(
+      Dafny.Aws.Cryptography.DynamoDbEncryption.Types.BatchExecuteStatementInputTransformInput dafnyValue) {
+    BatchExecuteStatementInputTransformInput.Builder nativeBuilder = BatchExecuteStatementInputTransformInput.builder();
+    nativeBuilder.sdkInput(Dafny.Com.Amazonaws.Dynamodb.ToNative.BatchExecuteStatementInput(dafnyValue.dtor_sdkInput()));
+    return nativeBuilder.build();
+  }
+
+  public static ConstructorPart ConstructorPart(
+      Dafny.Aws.Cryptography.DynamoDbEncryption.Types.ConstructorPart dafnyValue) {
+    ConstructorPart.Builder nativeBuilder = ConstructorPart.builder();
+    nativeBuilder.name(software.amazon.dafny.conversion.ToNative.Simple.String(dafnyValue.dtor_name()));
+    nativeBuilder.required((dafnyValue.dtor_required()));
+    return nativeBuilder.build();
+  }
+
+  public static BatchWriteItemOutputTransformOutput BatchWriteItemOutputTransformOutput(
+      Dafny.Aws.Cryptography.DynamoDbEncryption.Types.BatchWriteItemOutputTransformOutput dafnyValue) {
+    BatchWriteItemOutputTransformOutput.Builder nativeBuilder = BatchWriteItemOutputTransformOutput.builder();
+    nativeBuilder.transformedOutput(Dafny.Com.Amazonaws.Dynamodb.ToNative.BatchWriteItemOutput(dafnyValue.dtor_transformedOutput()));
+    return nativeBuilder.build();
+  }
+
+  public static UpdateTableInputTransformInput UpdateTableInputTransformInput(
+      Dafny.Aws.Cryptography.DynamoDbEncryption.Types.UpdateTableInputTransformInput dafnyValue) {
+    UpdateTableInputTransformInput.Builder nativeBuilder = UpdateTableInputTransformInput.builder();
+    nativeBuilder.sdkInput(Dafny.Com.Amazonaws.Dynamodb.ToNative.UpdateTableInput(dafnyValue.dtor_sdkInput()));
+    return nativeBuilder.build();
+  }
+
+  public static PutItemInputTransformInput PutItemInputTransformInput(
+      Dafny.Aws.Cryptography.DynamoDbEncryption.Types.PutItemInputTransformInput dafnyValue) {
+    PutItemInputTransformInput.Builder nativeBuilder = PutItemInputTransformInput.builder();
+    nativeBuilder.sdkInput(Dafny.Com.Amazonaws.Dynamodb.ToNative.PutItemInput(dafnyValue.dtor_sdkInput()));
+    return nativeBuilder.build();
+  }
+
+  public static BatchExecuteStatementOutputTransformOutput BatchExecuteStatementOutputTransformOutput(
+      Dafny.Aws.Cryptography.DynamoDbEncryption.Types.BatchExecuteStatementOutputTransformOutput dafnyValue) {
+    BatchExecuteStatementOutputTransformOutput.Builder nativeBuilder = BatchExecuteStatementOutputTransformOutput.builder();
+    nativeBuilder.transformedOutput(Dafny.Com.Amazonaws.Dynamodb.ToNative.BatchExecuteStatementOutput(dafnyValue.dtor_transformedOutput()));
+    return nativeBuilder.build();
+  }
+
+  public static ExecuteTransactionOutputTransformOutput ExecuteTransactionOutputTransformOutput(
+      Dafny.Aws.Cryptography.DynamoDbEncryption.Types.ExecuteTransactionOutputTransformOutput dafnyValue) {
+    ExecuteTransactionOutputTransformOutput.Builder nativeBuilder = ExecuteTransactionOutputTransformOutput.builder();
+    nativeBuilder.transformedOutput(Dafny.Com.Amazonaws.Dynamodb.ToNative.ExecuteTransactionOutput(dafnyValue.dtor_transformedOutput()));
+    return nativeBuilder.build();
+  }
+
+  public static TransactWriteItemsOutputTransformOutput TransactWriteItemsOutputTransformOutput(
+      Dafny.Aws.Cryptography.DynamoDbEncryption.Types.TransactWriteItemsOutputTransformOutput dafnyValue) {
+    TransactWriteItemsOutputTransformOutput.Builder nativeBuilder = TransactWriteItemsOutputTransformOutput.builder();
+    nativeBuilder.transformedOutput(Dafny.Com.Amazonaws.Dynamodb.ToNative.TransactWriteItemsOutput(dafnyValue.dtor_transformedOutput()));
+    return nativeBuilder.build();
+  }
+
+  public static GetItemInputTransformInput GetItemInputTransformInput(
+      Dafny.Aws.Cryptography.DynamoDbEncryption.Types.GetItemInputTransformInput dafnyValue) {
+    GetItemInputTransformInput.Builder nativeBuilder = GetItemInputTransformInput.builder();
+    nativeBuilder.sdkInput(Dafny.Com.Amazonaws.Dynamodb.ToNative.GetItemInput(dafnyValue.dtor_sdkInput()));
+    return nativeBuilder.build();
+  }
+
+  public static UpdateTableInputTransformOutput UpdateTableInputTransformOutput(
+      Dafny.Aws.Cryptography.DynamoDbEncryption.Types.UpdateTableInputTransformOutput dafnyValue) {
+    UpdateTableInputTransformOutput.Builder nativeBuilder = UpdateTableInputTransformOutput.builder();
+    nativeBuilder.transformedInput(Dafny.Com.Amazonaws.Dynamodb.ToNative.UpdateTableInput(dafnyValue.dtor_transformedInput()));
+    return nativeBuilder.build();
+  }
+
+  public static ExecuteStatementOutputTransformInput ExecuteStatementOutputTransformInput(
+      Dafny.Aws.Cryptography.DynamoDbEncryption.Types.ExecuteStatementOutputTransformInput dafnyValue) {
+    ExecuteStatementOutputTransformInput.Builder nativeBuilder = ExecuteStatementOutputTransformInput.builder();
+    nativeBuilder.sdkOutput(Dafny.Com.Amazonaws.Dynamodb.ToNative.ExecuteStatementOutput(dafnyValue.dtor_sdkOutput()));
+    nativeBuilder.originalInput(Dafny.Com.Amazonaws.Dynamodb.ToNative.ExecuteStatementInput(dafnyValue.dtor_originalInput()));
+    return nativeBuilder.build();
+  }
+
+  public static GetItemOutputTransformOutput GetItemOutputTransformOutput(
+      Dafny.Aws.Cryptography.DynamoDbEncryption.Types.GetItemOutputTransformOutput dafnyValue) {
+    GetItemOutputTransformOutput.Builder nativeBuilder = GetItemOutputTransformOutput.builder();
+    nativeBuilder.transformedOutput(Dafny.Com.Amazonaws.Dynamodb.ToNative.GetItemOutput(dafnyValue.dtor_transformedOutput()));
+    return nativeBuilder.build();
+  }
+
+  public static PutItemOutputTransformInput PutItemOutputTransformInput(
+      Dafny.Aws.Cryptography.DynamoDbEncryption.Types.PutItemOutputTransformInput dafnyValue) {
+    PutItemOutputTransformInput.Builder nativeBuilder = PutItemOutputTransformInput.builder();
+    nativeBuilder.sdkOutput(Dafny.Com.Amazonaws.Dynamodb.ToNative.PutItemOutput(dafnyValue.dtor_sdkOutput()));
+    nativeBuilder.originalInput(Dafny.Com.Amazonaws.Dynamodb.ToNative.PutItemInput(dafnyValue.dtor_originalInput()));
+    return nativeBuilder.build();
+  }
+
+  public static StandardBeacon StandardBeacon(
+      Dafny.Aws.Cryptography.DynamoDbEncryption.Types.StandardBeacon dafnyValue) {
+    StandardBeacon.Builder nativeBuilder = StandardBeacon.builder();
+    nativeBuilder.name(software.amazon.dafny.conversion.ToNative.Simple.String(dafnyValue.dtor_name()));
+    nativeBuilder.length((dafnyValue.dtor_length()));
+    if (dafnyValue.dtor_loc().is_Some()) {
+      nativeBuilder.loc(software.amazon.dafny.conversion.ToNative.Simple.String(dafnyValue.dtor_loc().dtor_value()));
+    }
+    return nativeBuilder.build();
+  }
+
+  public static BatchWriteItemInputTransformOutput BatchWriteItemInputTransformOutput(
+      Dafny.Aws.Cryptography.DynamoDbEncryption.Types.BatchWriteItemInputTransformOutput dafnyValue) {
+    BatchWriteItemInputTransformOutput.Builder nativeBuilder = BatchWriteItemInputTransformOutput.builder();
+    nativeBuilder.transformedInput(Dafny.Com.Amazonaws.Dynamodb.ToNative.BatchWriteItemInput(dafnyValue.dtor_transformedInput()));
+    return nativeBuilder.build();
+  }
+
+  public static UpdateTableOutputTransformInput UpdateTableOutputTransformInput(
+      Dafny.Aws.Cryptography.DynamoDbEncryption.Types.UpdateTableOutputTransformInput dafnyValue) {
+    UpdateTableOutputTransformInput.Builder nativeBuilder = UpdateTableOutputTransformInput.builder();
+    nativeBuilder.sdkOutput(Dafny.Com.Amazonaws.Dynamodb.ToNative.UpdateTableOutput(dafnyValue.dtor_sdkOutput()));
+    nativeBuilder.originalInput(Dafny.Com.Amazonaws.Dynamodb.ToNative.UpdateTableInput(dafnyValue.dtor_originalInput()));
+    return nativeBuilder.build();
+  }
+
+  public static Constructor Constructor(
+      Dafny.Aws.Cryptography.DynamoDbEncryption.Types.Constructor dafnyValue) {
+    Constructor.Builder nativeBuilder = Constructor.builder();
+    nativeBuilder.parts(ToNative.ConstructorPartList(dafnyValue.dtor_parts()));
+    return nativeBuilder.build();
+  }
+
+  public static PutItemOutputTransformOutput PutItemOutputTransformOutput(
+      Dafny.Aws.Cryptography.DynamoDbEncryption.Types.PutItemOutputTransformOutput dafnyValue) {
+    PutItemOutputTransformOutput.Builder nativeBuilder = PutItemOutputTransformOutput.builder();
+    nativeBuilder.transformedOutput(Dafny.Com.Amazonaws.Dynamodb.ToNative.PutItemOutput(dafnyValue.dtor_transformedOutput()));
+    return nativeBuilder.build();
+  }
+
+  public static BatchGetItemOutputTransformOutput BatchGetItemOutputTransformOutput(
+      Dafny.Aws.Cryptography.DynamoDbEncryption.Types.BatchGetItemOutputTransformOutput dafnyValue) {
+    BatchGetItemOutputTransformOutput.Builder nativeBuilder = BatchGetItemOutputTransformOutput.builder();
+    nativeBuilder.transformedOutput(Dafny.Com.Amazonaws.Dynamodb.ToNative.BatchGetItemOutput(dafnyValue.dtor_transformedOutput()));
+    return nativeBuilder.build();
+  }
+
+  public static UpdateItemInputTransformInput UpdateItemInputTransformInput(
+      Dafny.Aws.Cryptography.DynamoDbEncryption.Types.UpdateItemInputTransformInput dafnyValue) {
+    UpdateItemInputTransformInput.Builder nativeBuilder = UpdateItemInputTransformInput.builder();
+    nativeBuilder.sdkInput(Dafny.Com.Amazonaws.Dynamodb.ToNative.UpdateItemInput(dafnyValue.dtor_sdkInput()));
+    return nativeBuilder.build();
+  }
+
+  public static TransactGetItemsInputTransformInput TransactGetItemsInputTransformInput(
+      Dafny.Aws.Cryptography.DynamoDbEncryption.Types.TransactGetItemsInputTransformInput dafnyValue) {
+    TransactGetItemsInputTransformInput.Builder nativeBuilder = TransactGetItemsInputTransformInput.builder();
+    nativeBuilder.sdkInput(Dafny.Com.Amazonaws.Dynamodb.ToNative.TransactGetItemsInput(dafnyValue.dtor_sdkInput()));
+    return nativeBuilder.build();
+  }
+
+  public static BatchExecuteStatementOutputTransformInput BatchExecuteStatementOutputTransformInput(
+      Dafny.Aws.Cryptography.DynamoDbEncryption.Types.BatchExecuteStatementOutputTransformInput dafnyValue) {
+    BatchExecuteStatementOutputTransformInput.Builder nativeBuilder = BatchExecuteStatementOutputTransformInput.builder();
+    nativeBuilder.sdkOutput(Dafny.Com.Amazonaws.Dynamodb.ToNative.BatchExecuteStatementOutput(dafnyValue.dtor_sdkOutput()));
+    nativeBuilder.originalInput(Dafny.Com.Amazonaws.Dynamodb.ToNative.BatchExecuteStatementInput(dafnyValue.dtor_originalInput()));
+    return nativeBuilder.build();
+  }
+
+  public static BatchGetItemInputTransformOutput BatchGetItemInputTransformOutput(
+      Dafny.Aws.Cryptography.DynamoDbEncryption.Types.BatchGetItemInputTransformOutput dafnyValue) {
+    BatchGetItemInputTransformOutput.Builder nativeBuilder = BatchGetItemInputTransformOutput.builder();
+    nativeBuilder.transformedInput(Dafny.Com.Amazonaws.Dynamodb.ToNative.BatchGetItemInput(dafnyValue.dtor_transformedInput()));
+    return nativeBuilder.build();
+  }
+
+  public static UpdateItemOutputTransformInput UpdateItemOutputTransformInput(
+      Dafny.Aws.Cryptography.DynamoDbEncryption.Types.UpdateItemOutputTransformInput dafnyValue) {
+    UpdateItemOutputTransformInput.Builder nativeBuilder = UpdateItemOutputTransformInput.builder();
+    nativeBuilder.sdkOutput(Dafny.Com.Amazonaws.Dynamodb.ToNative.UpdateItemOutput(dafnyValue.dtor_sdkOutput()));
+    nativeBuilder.originalInput(Dafny.Com.Amazonaws.Dynamodb.ToNative.UpdateItemInput(dafnyValue.dtor_originalInput()));
+    return nativeBuilder.build();
+  }
+
+  public static ScanOutputTransformOutput ScanOutputTransformOutput(
+      Dafny.Aws.Cryptography.DynamoDbEncryption.Types.ScanOutputTransformOutput dafnyValue) {
+    ScanOutputTransformOutput.Builder nativeBuilder = ScanOutputTransformOutput.builder();
+    nativeBuilder.transformedOutput(Dafny.Com.Amazonaws.Dynamodb.ToNative.ScanOutput(dafnyValue.dtor_transformedOutput()));
+    return nativeBuilder.build();
+  }
+
+  public static QueryInputTransformInput QueryInputTransformInput(
+      Dafny.Aws.Cryptography.DynamoDbEncryption.Types.QueryInputTransformInput dafnyValue) {
+    QueryInputTransformInput.Builder nativeBuilder = QueryInputTransformInput.builder();
+    nativeBuilder.sdkInput(Dafny.Com.Amazonaws.Dynamodb.ToNative.QueryInput(dafnyValue.dtor_sdkInput()));
+    return nativeBuilder.build();
+  }
+
+  public static DeleteItemInputTransformOutput DeleteItemInputTransformOutput(
+      Dafny.Aws.Cryptography.DynamoDbEncryption.Types.DeleteItemInputTransformOutput dafnyValue) {
+    DeleteItemInputTransformOutput.Builder nativeBuilder = DeleteItemInputTransformOutput.builder();
+    nativeBuilder.transformedInput(Dafny.Com.Amazonaws.Dynamodb.ToNative.DeleteItemInput(dafnyValue.dtor_transformedInput()));
+    return nativeBuilder.build();
+  }
+
+  public static BatchWriteItemOutputTransformInput BatchWriteItemOutputTransformInput(
+      Dafny.Aws.Cryptography.DynamoDbEncryption.Types.BatchWriteItemOutputTransformInput dafnyValue) {
+    BatchWriteItemOutputTransformInput.Builder nativeBuilder = BatchWriteItemOutputTransformInput.builder();
+    nativeBuilder.sdkOutput(Dafny.Com.Amazonaws.Dynamodb.ToNative.BatchWriteItemOutput(dafnyValue.dtor_sdkOutput()));
+    nativeBuilder.originalInput(Dafny.Com.Amazonaws.Dynamodb.ToNative.BatchWriteItemInput(dafnyValue.dtor_originalInput()));
+    return nativeBuilder.build();
+  }
+
+  public static UpdateItemOutputTransformOutput UpdateItemOutputTransformOutput(
+      Dafny.Aws.Cryptography.DynamoDbEncryption.Types.UpdateItemOutputTransformOutput dafnyValue) {
+    UpdateItemOutputTransformOutput.Builder nativeBuilder = UpdateItemOutputTransformOutput.builder();
+    nativeBuilder.transformedOutput(Dafny.Com.Amazonaws.Dynamodb.ToNative.UpdateItemOutput(dafnyValue.dtor_transformedOutput()));
+    return nativeBuilder.build();
+  }
+
+  public static SensitivePart SensitivePart(
+      Dafny.Aws.Cryptography.DynamoDbEncryption.Types.SensitivePart dafnyValue) {
+    SensitivePart.Builder nativeBuilder = SensitivePart.builder();
+    nativeBuilder.name(software.amazon.dafny.conversion.ToNative.Simple.String(dafnyValue.dtor_name()));
+    nativeBuilder.prefix(software.amazon.dafny.conversion.ToNative.Simple.String(dafnyValue.dtor_prefix()));
+    nativeBuilder.length((dafnyValue.dtor_length()));
+    if (dafnyValue.dtor_loc().is_Some()) {
+      nativeBuilder.loc(software.amazon.dafny.conversion.ToNative.Simple.String(dafnyValue.dtor_loc().dtor_value()));
+    }
+    return nativeBuilder.build();
+  }
+
+  public static UpdateItemInputTransformOutput UpdateItemInputTransformOutput(
+      Dafny.Aws.Cryptography.DynamoDbEncryption.Types.UpdateItemInputTransformOutput dafnyValue) {
+    UpdateItemInputTransformOutput.Builder nativeBuilder = UpdateItemInputTransformOutput.builder();
+    nativeBuilder.transformedInput(Dafny.Com.Amazonaws.Dynamodb.ToNative.UpdateItemInput(dafnyValue.dtor_transformedInput()));
+    return nativeBuilder.build();
+  }
+
+  public static UpdateTableOutputTransformOutput UpdateTableOutputTransformOutput(
+      Dafny.Aws.Cryptography.DynamoDbEncryption.Types.UpdateTableOutputTransformOutput dafnyValue) {
+    UpdateTableOutputTransformOutput.Builder nativeBuilder = UpdateTableOutputTransformOutput.builder();
+    nativeBuilder.transformedOutput(Dafny.Com.Amazonaws.Dynamodb.ToNative.UpdateTableOutput(dafnyValue.dtor_transformedOutput()));
+    return nativeBuilder.build();
+  }
+
+  public static ScanInputTransformOutput ScanInputTransformOutput(
+      Dafny.Aws.Cryptography.DynamoDbEncryption.Types.ScanInputTransformOutput dafnyValue) {
+    ScanInputTransformOutput.Builder nativeBuilder = ScanInputTransformOutput.builder();
+    nativeBuilder.transformedInput(Dafny.Com.Amazonaws.Dynamodb.ToNative.ScanInput(dafnyValue.dtor_transformedInput()));
+    return nativeBuilder.build();
+  }
+
+  public static CompoundBeacon CompoundBeacon(
+      Dafny.Aws.Cryptography.DynamoDbEncryption.Types.CompoundBeacon dafnyValue) {
+    CompoundBeacon.Builder nativeBuilder = CompoundBeacon.builder();
+    nativeBuilder.name(software.amazon.dafny.conversion.ToNative.Simple.String(dafnyValue.dtor_name()));
+    nativeBuilder.split(software.amazon.dafny.conversion.ToNative.Simple.String(dafnyValue.dtor_split()));
+    nativeBuilder.sensitive(ToNative.SensitivePartsList(dafnyValue.dtor_sensitive()));
+    if (dafnyValue.dtor_nonSensitive().is_Some()) {
+      nativeBuilder.nonSensitive(ToNative.NonSensitivePartsList(dafnyValue.dtor_nonSensitive().dtor_value()));
+    }
+    if (dafnyValue.dtor_constructors().is_Some()) {
+      nativeBuilder.constructors(ToNative.ConstructorList(dafnyValue.dtor_constructors().dtor_value()));
+    }
+    return nativeBuilder.build();
+  }
+
+  public static VirtualField VirtualField(
+      Dafny.Aws.Cryptography.DynamoDbEncryption.Types.VirtualField dafnyValue) {
+    VirtualField.Builder nativeBuilder = VirtualField.builder();
+    nativeBuilder.name(software.amazon.dafny.conversion.ToNative.Simple.String(dafnyValue.dtor_name()));
+    nativeBuilder.parts(ToNative.VirtualPartList(dafnyValue.dtor_parts()));
+    return nativeBuilder.build();
+  }
+
+  public static BatchWriteItemInputTransformInput BatchWriteItemInputTransformInput(
+      Dafny.Aws.Cryptography.DynamoDbEncryption.Types.BatchWriteItemInputTransformInput dafnyValue) {
+    BatchWriteItemInputTransformInput.Builder nativeBuilder = BatchWriteItemInputTransformInput.builder();
+    nativeBuilder.sdkInput(Dafny.Com.Amazonaws.Dynamodb.ToNative.BatchWriteItemInput(dafnyValue.dtor_sdkInput()));
+    return nativeBuilder.build();
+  }
+
+  public static TransactWriteItemsInputTransformOutput TransactWriteItemsInputTransformOutput(
+      Dafny.Aws.Cryptography.DynamoDbEncryption.Types.TransactWriteItemsInputTransformOutput dafnyValue) {
+    TransactWriteItemsInputTransformOutput.Builder nativeBuilder = TransactWriteItemsInputTransformOutput.builder();
+    nativeBuilder.transformedInput(Dafny.Com.Amazonaws.Dynamodb.ToNative.TransactWriteItemsInput(dafnyValue.dtor_transformedInput()));
+    return nativeBuilder.build();
+  }
+
+  public static BatchGetItemOutputTransformInput BatchGetItemOutputTransformInput(
+      Dafny.Aws.Cryptography.DynamoDbEncryption.Types.BatchGetItemOutputTransformInput dafnyValue) {
+    BatchGetItemOutputTransformInput.Builder nativeBuilder = BatchGetItemOutputTransformInput.builder();
+    nativeBuilder.sdkOutput(Dafny.Com.Amazonaws.Dynamodb.ToNative.BatchGetItemOutput(dafnyValue.dtor_sdkOutput()));
+    nativeBuilder.originalInput(Dafny.Com.Amazonaws.Dynamodb.ToNative.BatchGetItemInput(dafnyValue.dtor_originalInput()));
+    return nativeBuilder.build();
+  }
+
+  public static ExecuteStatementOutputTransformOutput ExecuteStatementOutputTransformOutput(
+      Dafny.Aws.Cryptography.DynamoDbEncryption.Types.ExecuteStatementOutputTransformOutput dafnyValue) {
+    ExecuteStatementOutputTransformOutput.Builder nativeBuilder = ExecuteStatementOutputTransformOutput.builder();
+    nativeBuilder.transformedOutput(Dafny.Com.Amazonaws.Dynamodb.ToNative.ExecuteStatementOutput(dafnyValue.dtor_transformedOutput()));
+    return nativeBuilder.build();
+  }
+
+  public static SearchConfig SearchConfig(
+      Dafny.Aws.Cryptography.DynamoDbEncryption.Types.SearchConfig dafnyValue) {
+    SearchConfig.Builder nativeBuilder = SearchConfig.builder();
+    nativeBuilder.versions(ToNative.BeaconVersionList(dafnyValue.dtor_versions()));
+    nativeBuilder.writeVersion((dafnyValue.dtor_writeVersion()));
+    return nativeBuilder.build();
+  }
+
+  public static QueryOutputTransformOutput QueryOutputTransformOutput(
+      Dafny.Aws.Cryptography.DynamoDbEncryption.Types.QueryOutputTransformOutput dafnyValue) {
+    QueryOutputTransformOutput.Builder nativeBuilder = QueryOutputTransformOutput.builder();
+    nativeBuilder.transformedOutput(Dafny.Com.Amazonaws.Dynamodb.ToNative.QueryOutput(dafnyValue.dtor_transformedOutput()));
+    return nativeBuilder.build();
+  }
+
+  public static BatchGetItemInputTransformInput BatchGetItemInputTransformInput(
+      Dafny.Aws.Cryptography.DynamoDbEncryption.Types.BatchGetItemInputTransformInput dafnyValue) {
+    BatchGetItemInputTransformInput.Builder nativeBuilder = BatchGetItemInputTransformInput.builder();
+    nativeBuilder.sdkInput(Dafny.Com.Amazonaws.Dynamodb.ToNative.BatchGetItemInput(dafnyValue.dtor_sdkInput()));
+    return nativeBuilder.build();
+  }
+
+  public static NonSensitivePart NonSensitivePart(
+      Dafny.Aws.Cryptography.DynamoDbEncryption.Types.NonSensitivePart dafnyValue) {
+    NonSensitivePart.Builder nativeBuilder = NonSensitivePart.builder();
+    nativeBuilder.name(software.amazon.dafny.conversion.ToNative.Simple.String(dafnyValue.dtor_name()));
+    nativeBuilder.prefix(software.amazon.dafny.conversion.ToNative.Simple.String(dafnyValue.dtor_prefix()));
+    if (dafnyValue.dtor_loc().is_Some()) {
+      nativeBuilder.loc(software.amazon.dafny.conversion.ToNative.Simple.String(dafnyValue.dtor_loc().dtor_value()));
+    }
+    return nativeBuilder.build();
+  }
+
+  public static DynamoDbEncryptionConfig DynamoDbEncryptionConfig(
+      Dafny.Aws.Cryptography.DynamoDbEncryption.Types.DynamoDbEncryptionConfig dafnyValue) {
+    DynamoDbEncryptionConfig.Builder nativeBuilder = DynamoDbEncryptionConfig.builder();
+    nativeBuilder.tableEncryptionConfigs(ToNative.DynamoDbTableEncryptionConfigs(dafnyValue.dtor_tableEncryptionConfigs()));
+    return nativeBuilder.build();
+  }
+
+  public static TransactWriteItemsInputTransformInput TransactWriteItemsInputTransformInput(
+      Dafny.Aws.Cryptography.DynamoDbEncryption.Types.TransactWriteItemsInputTransformInput dafnyValue) {
+    TransactWriteItemsInputTransformInput.Builder nativeBuilder = TransactWriteItemsInputTransformInput.builder();
+    nativeBuilder.sdkInput(Dafny.Com.Amazonaws.Dynamodb.ToNative.TransactWriteItemsInput(dafnyValue.dtor_sdkInput()));
+    return nativeBuilder.build();
+  }
+
+  public static BatchExecuteStatementInputTransformOutput BatchExecuteStatementInputTransformOutput(
+      Dafny.Aws.Cryptography.DynamoDbEncryption.Types.BatchExecuteStatementInputTransformOutput dafnyValue) {
+    BatchExecuteStatementInputTransformOutput.Builder nativeBuilder = BatchExecuteStatementInputTransformOutput.builder();
+    nativeBuilder.transformedInput(Dafny.Com.Amazonaws.Dynamodb.ToNative.BatchExecuteStatementInput(dafnyValue.dtor_transformedInput()));
     return nativeBuilder.build();
   }
 
@@ -173,99 +695,11 @@ public class ToNative {
     return nativeBuilder.build();
   }
 
-  public static CreateTableOutputTransformOutput CreateTableOutputTransformOutput(
-      Dafny.Aws.Cryptography.DynamoDbEncryption.Types.CreateTableOutputTransformOutput dafnyValue) {
-    CreateTableOutputTransformOutput.Builder nativeBuilder = CreateTableOutputTransformOutput.builder();
-    nativeBuilder.transformedOutput(Dafny.Com.Amazonaws.Dynamodb.ToNative.CreateTableOutput(dafnyValue.dtor_transformedOutput()));
-    return nativeBuilder.build();
-  }
-
-  public static GetItemOutputTransformOutput GetItemOutputTransformOutput(
-      Dafny.Aws.Cryptography.DynamoDbEncryption.Types.GetItemOutputTransformOutput dafnyValue) {
-    GetItemOutputTransformOutput.Builder nativeBuilder = GetItemOutputTransformOutput.builder();
-    nativeBuilder.transformedOutput(Dafny.Com.Amazonaws.Dynamodb.ToNative.GetItemOutput(dafnyValue.dtor_transformedOutput()));
-    return nativeBuilder.build();
-  }
-
-  public static PutItemInputTransformInput PutItemInputTransformInput(
-      Dafny.Aws.Cryptography.DynamoDbEncryption.Types.PutItemInputTransformInput dafnyValue) {
-    PutItemInputTransformInput.Builder nativeBuilder = PutItemInputTransformInput.builder();
-    nativeBuilder.sdkInput(Dafny.Com.Amazonaws.Dynamodb.ToNative.PutItemInput(dafnyValue.dtor_sdkInput()));
-    return nativeBuilder.build();
-  }
-
-  public static NonSensitivePart NonSensitivePart(
-      Dafny.Aws.Cryptography.DynamoDbEncryption.Types.NonSensitivePart dafnyValue) {
-    NonSensitivePart.Builder nativeBuilder = NonSensitivePart.builder();
-    nativeBuilder.name(software.amazon.dafny.conversion.ToNative.Simple.String(dafnyValue.dtor_name()));
-    nativeBuilder.prefix(software.amazon.dafny.conversion.ToNative.Simple.String(dafnyValue.dtor_prefix()));
-    if (dafnyValue.dtor_loc().is_Some()) {
-      nativeBuilder.loc(software.amazon.dafny.conversion.ToNative.Simple.String(dafnyValue.dtor_loc().dtor_value()));
-    }
-    return nativeBuilder.build();
-  }
-
-  public static TransactGetItemsInputTransformOutput TransactGetItemsInputTransformOutput(
-      Dafny.Aws.Cryptography.DynamoDbEncryption.Types.TransactGetItemsInputTransformOutput dafnyValue) {
-    TransactGetItemsInputTransformOutput.Builder nativeBuilder = TransactGetItemsInputTransformOutput.builder();
-    nativeBuilder.transformedInput(Dafny.Com.Amazonaws.Dynamodb.ToNative.TransactGetItemsInput(dafnyValue.dtor_transformedInput()));
-    return nativeBuilder.build();
-  }
-
-  public static QueryInputTransformOutput QueryInputTransformOutput(
-      Dafny.Aws.Cryptography.DynamoDbEncryption.Types.QueryInputTransformOutput dafnyValue) {
-    QueryInputTransformOutput.Builder nativeBuilder = QueryInputTransformOutput.builder();
-    nativeBuilder.transformedInput(Dafny.Com.Amazonaws.Dynamodb.ToNative.QueryInput(dafnyValue.dtor_transformedInput()));
-    return nativeBuilder.build();
-  }
-
-  public static GetItemInputTransformOutput GetItemInputTransformOutput(
-      Dafny.Aws.Cryptography.DynamoDbEncryption.Types.GetItemInputTransformOutput dafnyValue) {
-    GetItemInputTransformOutput.Builder nativeBuilder = GetItemInputTransformOutput.builder();
-    nativeBuilder.transformedInput(Dafny.Com.Amazonaws.Dynamodb.ToNative.GetItemInput(dafnyValue.dtor_transformedInput()));
-    return nativeBuilder.build();
-  }
-
-  public static ExecuteTransactionInputTransformOutput ExecuteTransactionInputTransformOutput(
-      Dafny.Aws.Cryptography.DynamoDbEncryption.Types.ExecuteTransactionInputTransformOutput dafnyValue) {
-    ExecuteTransactionInputTransformOutput.Builder nativeBuilder = ExecuteTransactionInputTransformOutput.builder();
-    nativeBuilder.transformedInput(Dafny.Com.Amazonaws.Dynamodb.ToNative.ExecuteTransactionInput(dafnyValue.dtor_transformedInput()));
-    return nativeBuilder.build();
-  }
-
-  public static ExecuteStatementInputTransformInput ExecuteStatementInputTransformInput(
-      Dafny.Aws.Cryptography.DynamoDbEncryption.Types.ExecuteStatementInputTransformInput dafnyValue) {
-    ExecuteStatementInputTransformInput.Builder nativeBuilder = ExecuteStatementInputTransformInput.builder();
-    nativeBuilder.sdkInput(Dafny.Com.Amazonaws.Dynamodb.ToNative.ExecuteStatementInput(dafnyValue.dtor_sdkInput()));
-    return nativeBuilder.build();
-  }
-
-  public static BatchExecuteStatementInputTransformInput BatchExecuteStatementInputTransformInput(
-      Dafny.Aws.Cryptography.DynamoDbEncryption.Types.BatchExecuteStatementInputTransformInput dafnyValue) {
-    BatchExecuteStatementInputTransformInput.Builder nativeBuilder = BatchExecuteStatementInputTransformInput.builder();
-    nativeBuilder.sdkInput(Dafny.Com.Amazonaws.Dynamodb.ToNative.BatchExecuteStatementInput(dafnyValue.dtor_sdkInput()));
-    return nativeBuilder.build();
-  }
-
-  public static TransactGetItemsOutputTransformOutput TransactGetItemsOutputTransformOutput(
-      Dafny.Aws.Cryptography.DynamoDbEncryption.Types.TransactGetItemsOutputTransformOutput dafnyValue) {
-    TransactGetItemsOutputTransformOutput.Builder nativeBuilder = TransactGetItemsOutputTransformOutput.builder();
-    nativeBuilder.transformedOutput(Dafny.Com.Amazonaws.Dynamodb.ToNative.TransactGetItemsOutput(dafnyValue.dtor_transformedOutput()));
-    return nativeBuilder.build();
-  }
-
-  public static SearchConfig SearchConfig(
-      Dafny.Aws.Cryptography.DynamoDbEncryption.Types.SearchConfig dafnyValue) {
-    SearchConfig.Builder nativeBuilder = SearchConfig.builder();
-    nativeBuilder.versions(ToNative.BeaconVersionList(dafnyValue.dtor_versions()));
-    nativeBuilder.writeVersion((dafnyValue.dtor_writeVersion()));
-    return nativeBuilder.build();
-  }
-
-  public static PutItemInputTransformOutput PutItemInputTransformOutput(
-      Dafny.Aws.Cryptography.DynamoDbEncryption.Types.PutItemInputTransformOutput dafnyValue) {
-    PutItemInputTransformOutput.Builder nativeBuilder = PutItemInputTransformOutput.builder();
-    nativeBuilder.transformedInput(Dafny.Com.Amazonaws.Dynamodb.ToNative.PutItemInput(dafnyValue.dtor_transformedInput()));
+  public static DeleteItemOutputTransformInput DeleteItemOutputTransformInput(
+      Dafny.Aws.Cryptography.DynamoDbEncryption.Types.DeleteItemOutputTransformInput dafnyValue) {
+    DeleteItemOutputTransformInput.Builder nativeBuilder = DeleteItemOutputTransformInput.builder();
+    nativeBuilder.sdkOutput(Dafny.Com.Amazonaws.Dynamodb.ToNative.DeleteItemOutput(dafnyValue.dtor_sdkOutput()));
+    nativeBuilder.originalInput(Dafny.Com.Amazonaws.Dynamodb.ToNative.DeleteItemInput(dafnyValue.dtor_originalInput()));
     return nativeBuilder.build();
   }
 
@@ -277,25 +711,10 @@ public class ToNative {
     return nativeBuilder.build();
   }
 
-  public static DeleteItemInputTransformInput DeleteItemInputTransformInput(
-      Dafny.Aws.Cryptography.DynamoDbEncryption.Types.DeleteItemInputTransformInput dafnyValue) {
-    DeleteItemInputTransformInput.Builder nativeBuilder = DeleteItemInputTransformInput.builder();
-    nativeBuilder.sdkInput(Dafny.Com.Amazonaws.Dynamodb.ToNative.DeleteItemInput(dafnyValue.dtor_sdkInput()));
-    return nativeBuilder.build();
-  }
-
-  public static QueryOutputTransformInput QueryOutputTransformInput(
-      Dafny.Aws.Cryptography.DynamoDbEncryption.Types.QueryOutputTransformInput dafnyValue) {
-    QueryOutputTransformInput.Builder nativeBuilder = QueryOutputTransformInput.builder();
-    nativeBuilder.sdkOutput(Dafny.Com.Amazonaws.Dynamodb.ToNative.QueryOutput(dafnyValue.dtor_sdkOutput()));
-    nativeBuilder.originalInput(Dafny.Com.Amazonaws.Dynamodb.ToNative.QueryInput(dafnyValue.dtor_originalInput()));
-    return nativeBuilder.build();
-  }
-
-  public static GetItemInputTransformInput GetItemInputTransformInput(
-      Dafny.Aws.Cryptography.DynamoDbEncryption.Types.GetItemInputTransformInput dafnyValue) {
-    GetItemInputTransformInput.Builder nativeBuilder = GetItemInputTransformInput.builder();
-    nativeBuilder.sdkInput(Dafny.Com.Amazonaws.Dynamodb.ToNative.GetItemInput(dafnyValue.dtor_sdkInput()));
+  public static TransactGetItemsOutputTransformOutput TransactGetItemsOutputTransformOutput(
+      Dafny.Aws.Cryptography.DynamoDbEncryption.Types.TransactGetItemsOutputTransformOutput dafnyValue) {
+    TransactGetItemsOutputTransformOutput.Builder nativeBuilder = TransactGetItemsOutputTransformOutput.builder();
+    nativeBuilder.transformedOutput(Dafny.Com.Amazonaws.Dynamodb.ToNative.TransactGetItemsOutput(dafnyValue.dtor_transformedOutput()));
     return nativeBuilder.build();
   }
 
@@ -303,57 +722,6 @@ public class ToNative {
       Dafny.Aws.Cryptography.DynamoDbEncryption.Types.DescribeTableInputTransformInput dafnyValue) {
     DescribeTableInputTransformInput.Builder nativeBuilder = DescribeTableInputTransformInput.builder();
     nativeBuilder.sdkInput(Dafny.Com.Amazonaws.Dynamodb.ToNative.DescribeTableInput(dafnyValue.dtor_sdkInput()));
-    return nativeBuilder.build();
-  }
-
-  public static ScanInputTransformInput ScanInputTransformInput(
-      Dafny.Aws.Cryptography.DynamoDbEncryption.Types.ScanInputTransformInput dafnyValue) {
-    ScanInputTransformInput.Builder nativeBuilder = ScanInputTransformInput.builder();
-    nativeBuilder.sdkInput(Dafny.Com.Amazonaws.Dynamodb.ToNative.ScanInput(dafnyValue.dtor_sdkInput()));
-    return nativeBuilder.build();
-  }
-
-  public static UpdateTableOutputTransformOutput UpdateTableOutputTransformOutput(
-      Dafny.Aws.Cryptography.DynamoDbEncryption.Types.UpdateTableOutputTransformOutput dafnyValue) {
-    UpdateTableOutputTransformOutput.Builder nativeBuilder = UpdateTableOutputTransformOutput.builder();
-    nativeBuilder.transformedOutput(Dafny.Com.Amazonaws.Dynamodb.ToNative.UpdateTableOutput(dafnyValue.dtor_transformedOutput()));
-    return nativeBuilder.build();
-  }
-
-  public static DescribeTableOutputTransformOutput DescribeTableOutputTransformOutput(
-      Dafny.Aws.Cryptography.DynamoDbEncryption.Types.DescribeTableOutputTransformOutput dafnyValue) {
-    DescribeTableOutputTransformOutput.Builder nativeBuilder = DescribeTableOutputTransformOutput.builder();
-    nativeBuilder.transformedOutput(Dafny.Com.Amazonaws.Dynamodb.ToNative.DescribeTableOutput(dafnyValue.dtor_transformedOutput()));
-    return nativeBuilder.build();
-  }
-
-  public static DeleteItemOutputTransformOutput DeleteItemOutputTransformOutput(
-      Dafny.Aws.Cryptography.DynamoDbEncryption.Types.DeleteItemOutputTransformOutput dafnyValue) {
-    DeleteItemOutputTransformOutput.Builder nativeBuilder = DeleteItemOutputTransformOutput.builder();
-    nativeBuilder.transformedOutput(Dafny.Com.Amazonaws.Dynamodb.ToNative.DeleteItemOutput(dafnyValue.dtor_transformedOutput()));
-    return nativeBuilder.build();
-  }
-
-  public static GetItemOutputTransformInput GetItemOutputTransformInput(
-      Dafny.Aws.Cryptography.DynamoDbEncryption.Types.GetItemOutputTransformInput dafnyValue) {
-    GetItemOutputTransformInput.Builder nativeBuilder = GetItemOutputTransformInput.builder();
-    nativeBuilder.sdkOutput(Dafny.Com.Amazonaws.Dynamodb.ToNative.GetItemOutput(dafnyValue.dtor_sdkOutput()));
-    nativeBuilder.originalInput(Dafny.Com.Amazonaws.Dynamodb.ToNative.GetItemInput(dafnyValue.dtor_originalInput()));
-    return nativeBuilder.build();
-  }
-
-  public static TransactWriteItemsInputTransformOutput TransactWriteItemsInputTransformOutput(
-      Dafny.Aws.Cryptography.DynamoDbEncryption.Types.TransactWriteItemsInputTransformOutput dafnyValue) {
-    TransactWriteItemsInputTransformOutput.Builder nativeBuilder = TransactWriteItemsInputTransformOutput.builder();
-    nativeBuilder.transformedInput(Dafny.Com.Amazonaws.Dynamodb.ToNative.TransactWriteItemsInput(dafnyValue.dtor_transformedInput()));
-    return nativeBuilder.build();
-  }
-
-  public static BatchGetItemOutputTransformInput BatchGetItemOutputTransformInput(
-      Dafny.Aws.Cryptography.DynamoDbEncryption.Types.BatchGetItemOutputTransformInput dafnyValue) {
-    BatchGetItemOutputTransformInput.Builder nativeBuilder = BatchGetItemOutputTransformInput.builder();
-    nativeBuilder.sdkOutput(Dafny.Com.Amazonaws.Dynamodb.ToNative.BatchGetItemOutput(dafnyValue.dtor_sdkOutput()));
-    nativeBuilder.originalInput(Dafny.Com.Amazonaws.Dynamodb.ToNative.BatchGetItemInput(dafnyValue.dtor_originalInput()));
     return nativeBuilder.build();
   }
 
@@ -371,362 +739,57 @@ public class ToNative {
     return nativeBuilder.build();
   }
 
-  public static BatchGetItemInputTransformOutput BatchGetItemInputTransformOutput(
-      Dafny.Aws.Cryptography.DynamoDbEncryption.Types.BatchGetItemInputTransformOutput dafnyValue) {
-    BatchGetItemInputTransformOutput.Builder nativeBuilder = BatchGetItemInputTransformOutput.builder();
-    nativeBuilder.transformedInput(Dafny.Com.Amazonaws.Dynamodb.ToNative.BatchGetItemInput(dafnyValue.dtor_transformedInput()));
+  public static ScanInputTransformInput ScanInputTransformInput(
+      Dafny.Aws.Cryptography.DynamoDbEncryption.Types.ScanInputTransformInput dafnyValue) {
+    ScanInputTransformInput.Builder nativeBuilder = ScanInputTransformInput.builder();
+    nativeBuilder.sdkInput(Dafny.Com.Amazonaws.Dynamodb.ToNative.ScanInput(dafnyValue.dtor_sdkInput()));
     return nativeBuilder.build();
   }
 
-  public static BatchExecuteStatementOutputTransformInput BatchExecuteStatementOutputTransformInput(
-      Dafny.Aws.Cryptography.DynamoDbEncryption.Types.BatchExecuteStatementOutputTransformInput dafnyValue) {
-    BatchExecuteStatementOutputTransformInput.Builder nativeBuilder = BatchExecuteStatementOutputTransformInput.builder();
-    nativeBuilder.sdkOutput(Dafny.Com.Amazonaws.Dynamodb.ToNative.BatchExecuteStatementOutput(dafnyValue.dtor_sdkOutput()));
-    nativeBuilder.originalInput(Dafny.Com.Amazonaws.Dynamodb.ToNative.BatchExecuteStatementInput(dafnyValue.dtor_originalInput()));
+  public static DescribeTableOutputTransformOutput DescribeTableOutputTransformOutput(
+      Dafny.Aws.Cryptography.DynamoDbEncryption.Types.DescribeTableOutputTransformOutput dafnyValue) {
+    DescribeTableOutputTransformOutput.Builder nativeBuilder = DescribeTableOutputTransformOutput.builder();
+    nativeBuilder.transformedOutput(Dafny.Com.Amazonaws.Dynamodb.ToNative.DescribeTableOutput(dafnyValue.dtor_transformedOutput()));
     return nativeBuilder.build();
   }
 
-  public static DeleteItemOutputTransformInput DeleteItemOutputTransformInput(
-      Dafny.Aws.Cryptography.DynamoDbEncryption.Types.DeleteItemOutputTransformInput dafnyValue) {
-    DeleteItemOutputTransformInput.Builder nativeBuilder = DeleteItemOutputTransformInput.builder();
-    nativeBuilder.sdkOutput(Dafny.Com.Amazonaws.Dynamodb.ToNative.DeleteItemOutput(dafnyValue.dtor_sdkOutput()));
-    nativeBuilder.originalInput(Dafny.Com.Amazonaws.Dynamodb.ToNative.DeleteItemInput(dafnyValue.dtor_originalInput()));
-    return nativeBuilder.build();
-  }
-
-  public static DynamoDbEncryptionConfig DynamoDbEncryptionConfig(
-      Dafny.Aws.Cryptography.DynamoDbEncryption.Types.DynamoDbEncryptionConfig dafnyValue) {
-    DynamoDbEncryptionConfig.Builder nativeBuilder = DynamoDbEncryptionConfig.builder();
-    nativeBuilder.tableEncryptionConfigs(ToNative.DynamoDbTableEncryptionConfigs(dafnyValue.dtor_tableEncryptionConfigs()));
-    return nativeBuilder.build();
-  }
-
-  public static BatchExecuteStatementInputTransformOutput BatchExecuteStatementInputTransformOutput(
-      Dafny.Aws.Cryptography.DynamoDbEncryption.Types.BatchExecuteStatementInputTransformOutput dafnyValue) {
-    BatchExecuteStatementInputTransformOutput.Builder nativeBuilder = BatchExecuteStatementInputTransformOutput.builder();
-    nativeBuilder.transformedInput(Dafny.Com.Amazonaws.Dynamodb.ToNative.BatchExecuteStatementInput(dafnyValue.dtor_transformedInput()));
-    return nativeBuilder.build();
-  }
-
-  public static UpdateItemOutputTransformOutput UpdateItemOutputTransformOutput(
-      Dafny.Aws.Cryptography.DynamoDbEncryption.Types.UpdateItemOutputTransformOutput dafnyValue) {
-    UpdateItemOutputTransformOutput.Builder nativeBuilder = UpdateItemOutputTransformOutput.builder();
-    nativeBuilder.transformedOutput(Dafny.Com.Amazonaws.Dynamodb.ToNative.UpdateItemOutput(dafnyValue.dtor_transformedOutput()));
-    return nativeBuilder.build();
-  }
-
-  public static DeleteItemInputTransformOutput DeleteItemInputTransformOutput(
-      Dafny.Aws.Cryptography.DynamoDbEncryption.Types.DeleteItemInputTransformOutput dafnyValue) {
-    DeleteItemInputTransformOutput.Builder nativeBuilder = DeleteItemInputTransformOutput.builder();
-    nativeBuilder.transformedInput(Dafny.Com.Amazonaws.Dynamodb.ToNative.DeleteItemInput(dafnyValue.dtor_transformedInput()));
-    return nativeBuilder.build();
-  }
-
-  public static UpdateTableOutputTransformInput UpdateTableOutputTransformInput(
-      Dafny.Aws.Cryptography.DynamoDbEncryption.Types.UpdateTableOutputTransformInput dafnyValue) {
-    UpdateTableOutputTransformInput.Builder nativeBuilder = UpdateTableOutputTransformInput.builder();
-    nativeBuilder.sdkOutput(Dafny.Com.Amazonaws.Dynamodb.ToNative.UpdateTableOutput(dafnyValue.dtor_sdkOutput()));
-    nativeBuilder.originalInput(Dafny.Com.Amazonaws.Dynamodb.ToNative.UpdateTableInput(dafnyValue.dtor_originalInput()));
-    return nativeBuilder.build();
-  }
-
-  public static ExecuteStatementOutputTransformOutput ExecuteStatementOutputTransformOutput(
-      Dafny.Aws.Cryptography.DynamoDbEncryption.Types.ExecuteStatementOutputTransformOutput dafnyValue) {
-    ExecuteStatementOutputTransformOutput.Builder nativeBuilder = ExecuteStatementOutputTransformOutput.builder();
-    nativeBuilder.transformedOutput(Dafny.Com.Amazonaws.Dynamodb.ToNative.ExecuteStatementOutput(dafnyValue.dtor_transformedOutput()));
-    return nativeBuilder.build();
-  }
-
-  public static UpdateItemInputTransformOutput UpdateItemInputTransformOutput(
-      Dafny.Aws.Cryptography.DynamoDbEncryption.Types.UpdateItemInputTransformOutput dafnyValue) {
-    UpdateItemInputTransformOutput.Builder nativeBuilder = UpdateItemInputTransformOutput.builder();
-    nativeBuilder.transformedInput(Dafny.Com.Amazonaws.Dynamodb.ToNative.UpdateItemInput(dafnyValue.dtor_transformedInput()));
-    return nativeBuilder.build();
-  }
-
-  public static StandardBeacon StandardBeacon(
-      Dafny.Aws.Cryptography.DynamoDbEncryption.Types.StandardBeacon dafnyValue) {
-    StandardBeacon.Builder nativeBuilder = StandardBeacon.builder();
-    nativeBuilder.name(software.amazon.dafny.conversion.ToNative.Simple.String(dafnyValue.dtor_name()));
-    nativeBuilder.length((dafnyValue.dtor_length()));
-    if (dafnyValue.dtor_loc().is_Some()) {
-      nativeBuilder.loc(software.amazon.dafny.conversion.ToNative.Simple.String(dafnyValue.dtor_loc().dtor_value()));
+  public static Transform Transform(
+      Dafny.Aws.Cryptography.DynamoDbEncryption.Types.Transform dafnyValue) {
+    if (dafnyValue.is_LOWER()) {
+      return Transform.LOWER;
     }
-    return nativeBuilder.build();
-  }
-
-  public static ExecuteTransactionOutputTransformOutput ExecuteTransactionOutputTransformOutput(
-      Dafny.Aws.Cryptography.DynamoDbEncryption.Types.ExecuteTransactionOutputTransformOutput dafnyValue) {
-    ExecuteTransactionOutputTransformOutput.Builder nativeBuilder = ExecuteTransactionOutputTransformOutput.builder();
-    nativeBuilder.transformedOutput(Dafny.Com.Amazonaws.Dynamodb.ToNative.ExecuteTransactionOutput(dafnyValue.dtor_transformedOutput()));
-    return nativeBuilder.build();
-  }
-
-  public static SensitivePart SensitivePart(
-      Dafny.Aws.Cryptography.DynamoDbEncryption.Types.SensitivePart dafnyValue) {
-    SensitivePart.Builder nativeBuilder = SensitivePart.builder();
-    nativeBuilder.name(software.amazon.dafny.conversion.ToNative.Simple.String(dafnyValue.dtor_name()));
-    nativeBuilder.prefix(software.amazon.dafny.conversion.ToNative.Simple.String(dafnyValue.dtor_prefix()));
-    nativeBuilder.length((dafnyValue.dtor_length()));
-    if (dafnyValue.dtor_loc().is_Some()) {
-      nativeBuilder.loc(software.amazon.dafny.conversion.ToNative.Simple.String(dafnyValue.dtor_loc().dtor_value()));
+    if (dafnyValue.is_UPPER()) {
+      return Transform.UPPER;
     }
-    return nativeBuilder.build();
-  }
-
-  public static Constructor Constructor(
-      Dafny.Aws.Cryptography.DynamoDbEncryption.Types.Constructor dafnyValue) {
-    Constructor.Builder nativeBuilder = Constructor.builder();
-    nativeBuilder.parts(ToNative.ConstructorPartList(dafnyValue.dtor_parts()));
-    return nativeBuilder.build();
-  }
-
-  public static ConstructorPart ConstructorPart(
-      Dafny.Aws.Cryptography.DynamoDbEncryption.Types.ConstructorPart dafnyValue) {
-    ConstructorPart.Builder nativeBuilder = ConstructorPart.builder();
-    nativeBuilder.name(software.amazon.dafny.conversion.ToNative.Simple.String(dafnyValue.dtor_name()));
-    nativeBuilder.required((dafnyValue.dtor_required()));
-    return nativeBuilder.build();
-  }
-
-  public static UpdateTableInputTransformInput UpdateTableInputTransformInput(
-      Dafny.Aws.Cryptography.DynamoDbEncryption.Types.UpdateTableInputTransformInput dafnyValue) {
-    UpdateTableInputTransformInput.Builder nativeBuilder = UpdateTableInputTransformInput.builder();
-    nativeBuilder.sdkInput(Dafny.Com.Amazonaws.Dynamodb.ToNative.UpdateTableInput(dafnyValue.dtor_sdkInput()));
-    return nativeBuilder.build();
-  }
-
-  public static TransactGetItemsInputTransformInput TransactGetItemsInputTransformInput(
-      Dafny.Aws.Cryptography.DynamoDbEncryption.Types.TransactGetItemsInputTransformInput dafnyValue) {
-    TransactGetItemsInputTransformInput.Builder nativeBuilder = TransactGetItemsInputTransformInput.builder();
-    nativeBuilder.sdkInput(Dafny.Com.Amazonaws.Dynamodb.ToNative.TransactGetItemsInput(dafnyValue.dtor_sdkInput()));
-    return nativeBuilder.build();
-  }
-
-  public static PutItemOutputTransformOutput PutItemOutputTransformOutput(
-      Dafny.Aws.Cryptography.DynamoDbEncryption.Types.PutItemOutputTransformOutput dafnyValue) {
-    PutItemOutputTransformOutput.Builder nativeBuilder = PutItemOutputTransformOutput.builder();
-    nativeBuilder.transformedOutput(Dafny.Com.Amazonaws.Dynamodb.ToNative.PutItemOutput(dafnyValue.dtor_transformedOutput()));
-    return nativeBuilder.build();
-  }
-
-  public static QueryOutputTransformOutput QueryOutputTransformOutput(
-      Dafny.Aws.Cryptography.DynamoDbEncryption.Types.QueryOutputTransformOutput dafnyValue) {
-    QueryOutputTransformOutput.Builder nativeBuilder = QueryOutputTransformOutput.builder();
-    nativeBuilder.transformedOutput(Dafny.Com.Amazonaws.Dynamodb.ToNative.QueryOutput(dafnyValue.dtor_transformedOutput()));
-    return nativeBuilder.build();
-  }
-
-  public static UpdateItemInputTransformInput UpdateItemInputTransformInput(
-      Dafny.Aws.Cryptography.DynamoDbEncryption.Types.UpdateItemInputTransformInput dafnyValue) {
-    UpdateItemInputTransformInput.Builder nativeBuilder = UpdateItemInputTransformInput.builder();
-    nativeBuilder.sdkInput(Dafny.Com.Amazonaws.Dynamodb.ToNative.UpdateItemInput(dafnyValue.dtor_sdkInput()));
-    return nativeBuilder.build();
-  }
-
-  public static CompoundBeacon CompoundBeacon(
-      Dafny.Aws.Cryptography.DynamoDbEncryption.Types.CompoundBeacon dafnyValue) {
-    CompoundBeacon.Builder nativeBuilder = CompoundBeacon.builder();
-    nativeBuilder.name(software.amazon.dafny.conversion.ToNative.Simple.String(dafnyValue.dtor_name()));
-    nativeBuilder.split(software.amazon.dafny.conversion.ToNative.Simple.String(dafnyValue.dtor_split()));
-    nativeBuilder.sensitive(ToNative.SensitivePartsList(dafnyValue.dtor_sensitive()));
-    if (dafnyValue.dtor_nonSensitive().is_Some()) {
-      nativeBuilder.nonSensitive(ToNative.NonSensitivePartsList(dafnyValue.dtor_nonSensitive().dtor_value()));
+    if (dafnyValue.is_INSERT()) {
+      return Transform.INSERT;
     }
-    if (dafnyValue.dtor_constructors().is_Some()) {
-      nativeBuilder.constructors(ToNative.ConstructorList(dafnyValue.dtor_constructors().dtor_value()));
+    if (dafnyValue.is_PREFIX()) {
+      return Transform.PREFIX;
     }
-    return nativeBuilder.build();
+    if (dafnyValue.is_SUFFIX()) {
+      return Transform.SUFFIX;
+    }
+    if (dafnyValue.is_SUBSTRING()) {
+      return Transform.SUBSTRING;
+    }
+    if (dafnyValue.is_SEGMENT()) {
+      return Transform.SEGMENT;
+    }
+    throw new IllegalArgumentException("No entry of software.amazon.cryptography.dynamoDbEncryption.model.Transform matches the input : " + dafnyValue);
   }
 
-  public static BatchWriteItemOutputTransformOutput BatchWriteItemOutputTransformOutput(
-      Dafny.Aws.Cryptography.DynamoDbEncryption.Types.BatchWriteItemOutputTransformOutput dafnyValue) {
-    BatchWriteItemOutputTransformOutput.Builder nativeBuilder = BatchWriteItemOutputTransformOutput.builder();
-    nativeBuilder.transformedOutput(Dafny.Com.Amazonaws.Dynamodb.ToNative.BatchWriteItemOutput(dafnyValue.dtor_transformedOutput()));
-    return nativeBuilder.build();
-  }
-
-  public static ScanOutputTransformOutput ScanOutputTransformOutput(
-      Dafny.Aws.Cryptography.DynamoDbEncryption.Types.ScanOutputTransformOutput dafnyValue) {
-    ScanOutputTransformOutput.Builder nativeBuilder = ScanOutputTransformOutput.builder();
-    nativeBuilder.transformedOutput(Dafny.Com.Amazonaws.Dynamodb.ToNative.ScanOutput(dafnyValue.dtor_transformedOutput()));
-    return nativeBuilder.build();
-  }
-
-  public static TransactWriteItemsInputTransformInput TransactWriteItemsInputTransformInput(
-      Dafny.Aws.Cryptography.DynamoDbEncryption.Types.TransactWriteItemsInputTransformInput dafnyValue) {
-    TransactWriteItemsInputTransformInput.Builder nativeBuilder = TransactWriteItemsInputTransformInput.builder();
-    nativeBuilder.sdkInput(Dafny.Com.Amazonaws.Dynamodb.ToNative.TransactWriteItemsInput(dafnyValue.dtor_sdkInput()));
-    return nativeBuilder.build();
-  }
-
-  public static BatchGetItemInputTransformInput BatchGetItemInputTransformInput(
-      Dafny.Aws.Cryptography.DynamoDbEncryption.Types.BatchGetItemInputTransformInput dafnyValue) {
-    BatchGetItemInputTransformInput.Builder nativeBuilder = BatchGetItemInputTransformInput.builder();
-    nativeBuilder.sdkInput(Dafny.Com.Amazonaws.Dynamodb.ToNative.BatchGetItemInput(dafnyValue.dtor_sdkInput()));
-    return nativeBuilder.build();
-  }
-
-  public static UpdateItemOutputTransformInput UpdateItemOutputTransformInput(
-      Dafny.Aws.Cryptography.DynamoDbEncryption.Types.UpdateItemOutputTransformInput dafnyValue) {
-    UpdateItemOutputTransformInput.Builder nativeBuilder = UpdateItemOutputTransformInput.builder();
-    nativeBuilder.sdkOutput(Dafny.Com.Amazonaws.Dynamodb.ToNative.UpdateItemOutput(dafnyValue.dtor_sdkOutput()));
-    nativeBuilder.originalInput(Dafny.Com.Amazonaws.Dynamodb.ToNative.UpdateItemInput(dafnyValue.dtor_originalInput()));
-    return nativeBuilder.build();
-  }
-
-  public static UpdateTableInputTransformOutput UpdateTableInputTransformOutput(
-      Dafny.Aws.Cryptography.DynamoDbEncryption.Types.UpdateTableInputTransformOutput dafnyValue) {
-    UpdateTableInputTransformOutput.Builder nativeBuilder = UpdateTableInputTransformOutput.builder();
-    nativeBuilder.transformedInput(Dafny.Com.Amazonaws.Dynamodb.ToNative.UpdateTableInput(dafnyValue.dtor_transformedInput()));
-    return nativeBuilder.build();
-  }
-
-  public static QueryInputTransformInput QueryInputTransformInput(
-      Dafny.Aws.Cryptography.DynamoDbEncryption.Types.QueryInputTransformInput dafnyValue) {
-    QueryInputTransformInput.Builder nativeBuilder = QueryInputTransformInput.builder();
-    nativeBuilder.sdkInput(Dafny.Com.Amazonaws.Dynamodb.ToNative.QueryInput(dafnyValue.dtor_sdkInput()));
-    return nativeBuilder.build();
-  }
-
-  public static PutItemOutputTransformInput PutItemOutputTransformInput(
-      Dafny.Aws.Cryptography.DynamoDbEncryption.Types.PutItemOutputTransformInput dafnyValue) {
-    PutItemOutputTransformInput.Builder nativeBuilder = PutItemOutputTransformInput.builder();
-    nativeBuilder.sdkOutput(Dafny.Com.Amazonaws.Dynamodb.ToNative.PutItemOutput(dafnyValue.dtor_sdkOutput()));
-    nativeBuilder.originalInput(Dafny.Com.Amazonaws.Dynamodb.ToNative.PutItemInput(dafnyValue.dtor_originalInput()));
-    return nativeBuilder.build();
-  }
-
-  public static TransactGetItemsOutputTransformInput TransactGetItemsOutputTransformInput(
-      Dafny.Aws.Cryptography.DynamoDbEncryption.Types.TransactGetItemsOutputTransformInput dafnyValue) {
-    TransactGetItemsOutputTransformInput.Builder nativeBuilder = TransactGetItemsOutputTransformInput.builder();
-    nativeBuilder.sdkOutput(Dafny.Com.Amazonaws.Dynamodb.ToNative.TransactGetItemsOutput(dafnyValue.dtor_sdkOutput()));
-    nativeBuilder.originalInput(Dafny.Com.Amazonaws.Dynamodb.ToNative.TransactGetItemsInput(dafnyValue.dtor_originalInput()));
-    return nativeBuilder.build();
-  }
-
-  public static BatchWriteItemOutputTransformInput BatchWriteItemOutputTransformInput(
-      Dafny.Aws.Cryptography.DynamoDbEncryption.Types.BatchWriteItemOutputTransformInput dafnyValue) {
-    BatchWriteItemOutputTransformInput.Builder nativeBuilder = BatchWriteItemOutputTransformInput.builder();
-    nativeBuilder.sdkOutput(Dafny.Com.Amazonaws.Dynamodb.ToNative.BatchWriteItemOutput(dafnyValue.dtor_sdkOutput()));
-    nativeBuilder.originalInput(Dafny.Com.Amazonaws.Dynamodb.ToNative.BatchWriteItemInput(dafnyValue.dtor_originalInput()));
-    return nativeBuilder.build();
-  }
-
-  public static ScanInputTransformOutput ScanInputTransformOutput(
-      Dafny.Aws.Cryptography.DynamoDbEncryption.Types.ScanInputTransformOutput dafnyValue) {
-    ScanInputTransformOutput.Builder nativeBuilder = ScanInputTransformOutput.builder();
-    nativeBuilder.transformedInput(Dafny.Com.Amazonaws.Dynamodb.ToNative.ScanInput(dafnyValue.dtor_transformedInput()));
-    return nativeBuilder.build();
-  }
-
-  public static CreateTableOutputTransformInput CreateTableOutputTransformInput(
-      Dafny.Aws.Cryptography.DynamoDbEncryption.Types.CreateTableOutputTransformInput dafnyValue) {
-    CreateTableOutputTransformInput.Builder nativeBuilder = CreateTableOutputTransformInput.builder();
-    nativeBuilder.sdkOutput(Dafny.Com.Amazonaws.Dynamodb.ToNative.CreateTableOutput(dafnyValue.dtor_sdkOutput()));
-    nativeBuilder.originalInput(Dafny.Com.Amazonaws.Dynamodb.ToNative.CreateTableInput(dafnyValue.dtor_originalInput()));
-    return nativeBuilder.build();
-  }
-
-  public static ExecuteTransactionOutputTransformInput ExecuteTransactionOutputTransformInput(
-      Dafny.Aws.Cryptography.DynamoDbEncryption.Types.ExecuteTransactionOutputTransformInput dafnyValue) {
-    ExecuteTransactionOutputTransformInput.Builder nativeBuilder = ExecuteTransactionOutputTransformInput.builder();
-    nativeBuilder.sdkOutput(Dafny.Com.Amazonaws.Dynamodb.ToNative.ExecuteTransactionOutput(dafnyValue.dtor_sdkOutput()));
-    nativeBuilder.originalInput(Dafny.Com.Amazonaws.Dynamodb.ToNative.ExecuteTransactionInput(dafnyValue.dtor_originalInput()));
-    return nativeBuilder.build();
-  }
-
-  public static DescribeTableOutputTransformInput DescribeTableOutputTransformInput(
-      Dafny.Aws.Cryptography.DynamoDbEncryption.Types.DescribeTableOutputTransformInput dafnyValue) {
-    DescribeTableOutputTransformInput.Builder nativeBuilder = DescribeTableOutputTransformInput.builder();
-    nativeBuilder.sdkOutput(Dafny.Com.Amazonaws.Dynamodb.ToNative.DescribeTableOutput(dafnyValue.dtor_sdkOutput()));
-    nativeBuilder.originalInput(Dafny.Com.Amazonaws.Dynamodb.ToNative.DescribeTableInput(dafnyValue.dtor_originalInput()));
-    return nativeBuilder.build();
-  }
-
-  public static BatchWriteItemInputTransformInput BatchWriteItemInputTransformInput(
-      Dafny.Aws.Cryptography.DynamoDbEncryption.Types.BatchWriteItemInputTransformInput dafnyValue) {
-    BatchWriteItemInputTransformInput.Builder nativeBuilder = BatchWriteItemInputTransformInput.builder();
-    nativeBuilder.sdkInput(Dafny.Com.Amazonaws.Dynamodb.ToNative.BatchWriteItemInput(dafnyValue.dtor_sdkInput()));
-    return nativeBuilder.build();
-  }
-
-  public static DescribeTableInputTransformOutput DescribeTableInputTransformOutput(
-      Dafny.Aws.Cryptography.DynamoDbEncryption.Types.DescribeTableInputTransformOutput dafnyValue) {
-    DescribeTableInputTransformOutput.Builder nativeBuilder = DescribeTableInputTransformOutput.builder();
-    nativeBuilder.transformedInput(Dafny.Com.Amazonaws.Dynamodb.ToNative.DescribeTableInput(dafnyValue.dtor_transformedInput()));
-    return nativeBuilder.build();
-  }
-
-  public static ExecuteStatementInputTransformOutput ExecuteStatementInputTransformOutput(
-      Dafny.Aws.Cryptography.DynamoDbEncryption.Types.ExecuteStatementInputTransformOutput dafnyValue) {
-    ExecuteStatementInputTransformOutput.Builder nativeBuilder = ExecuteStatementInputTransformOutput.builder();
-    nativeBuilder.transformedInput(Dafny.Com.Amazonaws.Dynamodb.ToNative.ExecuteStatementInput(dafnyValue.dtor_transformedInput()));
-    return nativeBuilder.build();
-  }
-
-  public static BatchGetItemOutputTransformOutput BatchGetItemOutputTransformOutput(
-      Dafny.Aws.Cryptography.DynamoDbEncryption.Types.BatchGetItemOutputTransformOutput dafnyValue) {
-    BatchGetItemOutputTransformOutput.Builder nativeBuilder = BatchGetItemOutputTransformOutput.builder();
-    nativeBuilder.transformedOutput(Dafny.Com.Amazonaws.Dynamodb.ToNative.BatchGetItemOutput(dafnyValue.dtor_transformedOutput()));
-    return nativeBuilder.build();
-  }
-
-  public static CreateTableInputTransformOutput CreateTableInputTransformOutput(
-      Dafny.Aws.Cryptography.DynamoDbEncryption.Types.CreateTableInputTransformOutput dafnyValue) {
-    CreateTableInputTransformOutput.Builder nativeBuilder = CreateTableInputTransformOutput.builder();
-    nativeBuilder.transformedInput(Dafny.Com.Amazonaws.Dynamodb.ToNative.CreateTableInput(dafnyValue.dtor_transformedInput()));
-    return nativeBuilder.build();
-  }
-
-  public static BatchWriteItemInputTransformOutput BatchWriteItemInputTransformOutput(
-      Dafny.Aws.Cryptography.DynamoDbEncryption.Types.BatchWriteItemInputTransformOutput dafnyValue) {
-    BatchWriteItemInputTransformOutput.Builder nativeBuilder = BatchWriteItemInputTransformOutput.builder();
-    nativeBuilder.transformedInput(Dafny.Com.Amazonaws.Dynamodb.ToNative.BatchWriteItemInput(dafnyValue.dtor_transformedInput()));
-    return nativeBuilder.build();
-  }
-
-  public static BatchExecuteStatementOutputTransformOutput BatchExecuteStatementOutputTransformOutput(
-      Dafny.Aws.Cryptography.DynamoDbEncryption.Types.BatchExecuteStatementOutputTransformOutput dafnyValue) {
-    BatchExecuteStatementOutputTransformOutput.Builder nativeBuilder = BatchExecuteStatementOutputTransformOutput.builder();
-    nativeBuilder.transformedOutput(Dafny.Com.Amazonaws.Dynamodb.ToNative.BatchExecuteStatementOutput(dafnyValue.dtor_transformedOutput()));
-    return nativeBuilder.build();
-  }
-
-  public static ExecuteTransactionInputTransformInput ExecuteTransactionInputTransformInput(
-      Dafny.Aws.Cryptography.DynamoDbEncryption.Types.ExecuteTransactionInputTransformInput dafnyValue) {
-    ExecuteTransactionInputTransformInput.Builder nativeBuilder = ExecuteTransactionInputTransformInput.builder();
-    nativeBuilder.sdkInput(Dafny.Com.Amazonaws.Dynamodb.ToNative.ExecuteTransactionInput(dafnyValue.dtor_sdkInput()));
-    return nativeBuilder.build();
-  }
-
-  public static ExecuteStatementOutputTransformInput ExecuteStatementOutputTransformInput(
-      Dafny.Aws.Cryptography.DynamoDbEncryption.Types.ExecuteStatementOutputTransformInput dafnyValue) {
-    ExecuteStatementOutputTransformInput.Builder nativeBuilder = ExecuteStatementOutputTransformInput.builder();
-    nativeBuilder.sdkOutput(Dafny.Com.Amazonaws.Dynamodb.ToNative.ExecuteStatementOutput(dafnyValue.dtor_sdkOutput()));
-    nativeBuilder.originalInput(Dafny.Com.Amazonaws.Dynamodb.ToNative.ExecuteStatementInput(dafnyValue.dtor_originalInput()));
-    return nativeBuilder.build();
-  }
-
-  public static TransactWriteItemsOutputTransformOutput TransactWriteItemsOutputTransformOutput(
-      Dafny.Aws.Cryptography.DynamoDbEncryption.Types.TransactWriteItemsOutputTransformOutput dafnyValue) {
-    TransactWriteItemsOutputTransformOutput.Builder nativeBuilder = TransactWriteItemsOutputTransformOutput.builder();
-    nativeBuilder.transformedOutput(Dafny.Com.Amazonaws.Dynamodb.ToNative.TransactWriteItemsOutput(dafnyValue.dtor_transformedOutput()));
-    return nativeBuilder.build();
-  }
-
-  public static List<StandardBeacon> StandardBeaconList(
-      DafnySequence<? extends Dafny.Aws.Cryptography.DynamoDbEncryption.Types.StandardBeacon> dafnyValue) {
+  public static List<Integer> NumberList(DafnySequence<? extends Integer> dafnyValue) {
     return software.amazon.dafny.conversion.ToNative.Aggregate.GenericToList(
         dafnyValue, 
-        software.amazon.cryptography.dynamoDbEncryption.ToNative::StandardBeacon);
+        Function.identity());
   }
 
-  public static List<NonSensitivePart> NonSensitivePartsList(
-      DafnySequence<? extends Dafny.Aws.Cryptography.DynamoDbEncryption.Types.NonSensitivePart> dafnyValue) {
+  public static List<VirtualTransform> VirtualTransformList(
+      DafnySequence<? extends Dafny.Aws.Cryptography.DynamoDbEncryption.Types.VirtualTransform> dafnyValue) {
     return software.amazon.dafny.conversion.ToNative.Aggregate.GenericToList(
         dafnyValue, 
-        software.amazon.cryptography.dynamoDbEncryption.ToNative::NonSensitivePart);
+        software.amazon.cryptography.dynamoDbEncryption.ToNative::VirtualTransform);
   }
 
   public static List<SensitivePart> SensitivePartsList(
@@ -743,13 +806,6 @@ public class ToNative {
         software.amazon.cryptography.dynamoDbEncryption.ToNative::CompoundBeacon);
   }
 
-  public static List<Constructor> ConstructorList(
-      DafnySequence<? extends Dafny.Aws.Cryptography.DynamoDbEncryption.Types.Constructor> dafnyValue) {
-    return software.amazon.dafny.conversion.ToNative.Aggregate.GenericToList(
-        dafnyValue, 
-        software.amazon.cryptography.dynamoDbEncryption.ToNative::Constructor);
-  }
-
   public static List<BeaconVersion> BeaconVersionList(
       DafnySequence<? extends Dafny.Aws.Cryptography.DynamoDbEncryption.Types.BeaconVersion> dafnyValue) {
     return software.amazon.dafny.conversion.ToNative.Aggregate.GenericToList(
@@ -757,11 +813,53 @@ public class ToNative {
         software.amazon.cryptography.dynamoDbEncryption.ToNative::BeaconVersion);
   }
 
+  public static List<String> StringList(
+      DafnySequence<? extends DafnySequence<? extends Character>> dafnyValue) {
+    return software.amazon.dafny.conversion.ToNative.Aggregate.GenericToList(
+        dafnyValue, 
+        software.amazon.dafny.conversion.ToNative.Simple::String);
+  }
+
+  public static List<StandardBeacon> StandardBeaconList(
+      DafnySequence<? extends Dafny.Aws.Cryptography.DynamoDbEncryption.Types.StandardBeacon> dafnyValue) {
+    return software.amazon.dafny.conversion.ToNative.Aggregate.GenericToList(
+        dafnyValue, 
+        software.amazon.cryptography.dynamoDbEncryption.ToNative::StandardBeacon);
+  }
+
+  public static List<Constructor> ConstructorList(
+      DafnySequence<? extends Dafny.Aws.Cryptography.DynamoDbEncryption.Types.Constructor> dafnyValue) {
+    return software.amazon.dafny.conversion.ToNative.Aggregate.GenericToList(
+        dafnyValue, 
+        software.amazon.cryptography.dynamoDbEncryption.ToNative::Constructor);
+  }
+
   public static List<ConstructorPart> ConstructorPartList(
       DafnySequence<? extends Dafny.Aws.Cryptography.DynamoDbEncryption.Types.ConstructorPart> dafnyValue) {
     return software.amazon.dafny.conversion.ToNative.Aggregate.GenericToList(
         dafnyValue, 
         software.amazon.cryptography.dynamoDbEncryption.ToNative::ConstructorPart);
+  }
+
+  public static List<VirtualField> VirtualFieldList(
+      DafnySequence<? extends Dafny.Aws.Cryptography.DynamoDbEncryption.Types.VirtualField> dafnyValue) {
+    return software.amazon.dafny.conversion.ToNative.Aggregate.GenericToList(
+        dafnyValue, 
+        software.amazon.cryptography.dynamoDbEncryption.ToNative::VirtualField);
+  }
+
+  public static List<NonSensitivePart> NonSensitivePartsList(
+      DafnySequence<? extends Dafny.Aws.Cryptography.DynamoDbEncryption.Types.NonSensitivePart> dafnyValue) {
+    return software.amazon.dafny.conversion.ToNative.Aggregate.GenericToList(
+        dafnyValue, 
+        software.amazon.cryptography.dynamoDbEncryption.ToNative::NonSensitivePart);
+  }
+
+  public static List<VirtualPart> VirtualPartList(
+      DafnySequence<? extends Dafny.Aws.Cryptography.DynamoDbEncryption.Types.VirtualPart> dafnyValue) {
+    return software.amazon.dafny.conversion.ToNative.Aggregate.GenericToList(
+        dafnyValue, 
+        software.amazon.cryptography.dynamoDbEncryption.ToNative::VirtualPart);
   }
 
   public static Map<String, DynamoDbTableEncryptionConfig> DynamoDbTableEncryptionConfigs(
