DynamoDbEncryptionMiddlewareInternal/runtimes/java/src/main/smithy-generated/software/amazon/cryptography/dynamoDbEncryption/model/Transform.java
@@ -1,0 +1,30 @@
+// Copyright Amazon.com Inc. or its affiliates. All Rights Reserved.
+// SPDX-License-Identifier: Apache-2.0
+// Do not modify this file. This file is machine generated, and any changes to it will be overwritten.
+package software.amazon.cryptography.dynamoDbEncryption.model;
+
+public enum Transform {
+  LOWER("Lower"),
+
+  UPPER("Upper"),
+
+  INSERT("Insert"),
+
+  PREFIX("Prefix"),
+
+  SUFFIX("Suffix"),
+
+  SUBSTRING("Substring"),
+
+  SEGMENT("Segment");
+
+  private final String value;
+
+  private Transform(String value) {
+    this.value = value;
+  }
+
+  public String toString() {
+    return String.valueOf(value);
+  }
+}
