DynamoDbEncryptionMiddlewareInternal/runtimes/java/src/main/smithy-generated/software/amazon/cryptography/dynamoDbEncryption/model/VirtualTransform.java
@@ -1,0 +1,114 @@
+// Copyright Amazon.com Inc. or its affiliates. All Rights Reserved.
+// SPDX-License-Identifier: Apache-2.0
+// Do not modify this file. This file is machine generated, and any changes to it will be overwritten.
+package software.amazon.cryptography.dynamoDbEncryption.model;
+
+import java.util.List;
+import java.util.Objects;
+
+public class VirtualTransform {
+  private final Transform transform;
+
+  private final List<Integer> numbers;
+
+  private final List<String> strings;
+
+  protected VirtualTransform(BuilderImpl builder) {
+    this.transform = builder.transform();
+    this.numbers = builder.numbers();
+    this.strings = builder.strings();
+  }
+
+  public Transform transform() {
+    return this.transform;
+  }
+
+  public List<Integer> numbers() {
+    return this.numbers;
+  }
+
+  public List<String> strings() {
+    return this.strings;
+  }
+
+  public Builder toBuilder() {
+    return new BuilderImpl(this);
+  }
+
+  public static Builder builder() {
+    return new BuilderImpl();
+  }
+
+  public interface Builder {
+    Builder transform(Transform transform);
+
+    Transform transform();
+
+    Builder numbers(List<Integer> numbers);
+
+    List<Integer> numbers();
+
+    Builder strings(List<String> strings);
+
+    List<String> strings();
+
+    VirtualTransform build();
+  }
+
+  static class BuilderImpl implements Builder {
+    protected Transform transform;
+
+    protected List<Integer> numbers;
+
+    protected List<String> strings;
+
+    protected BuilderImpl() {
+    }
+
+    protected BuilderImpl(VirtualTransform model) {
+      this.transform = model.transform();
+      this.numbers = model.numbers();
+      this.strings = model.strings();
+    }
+
+    public Builder transform(Transform transform) {
+      this.transform = transform;
+      return this;
+    }
+
+    public Transform transform() {
+      return this.transform;
+    }
+
+    public Builder numbers(List<Integer> numbers) {
+      this.numbers = numbers;
+      return this;
+    }
+
+    public List<Integer> numbers() {
+      return this.numbers;
+    }
+
+    public Builder strings(List<String> strings) {
+      this.strings = strings;
+      return this;
+    }
+
+    public List<String> strings() {
+      return this.strings;
+    }
+
+    public VirtualTransform build() {
+      if (Objects.isNull(this.transform()))  {
+        throw new IllegalArgumentException("Missing value for required field `transform`");
+      }
+      if (Objects.nonNull(this.numbers()) && this.numbers().size() < 1) {
+        throw new IllegalArgumentException("The size of `numbers` must be greater than or equal to 1");
+      }
+      if (Objects.nonNull(this.strings()) && this.strings().size() < 1) {
+        throw new IllegalArgumentException("The size of `strings` must be greater than or equal to 1");
+      }
+      return new VirtualTransform(this);
+    }
+  }
+}
